changed EValue to contain an ext_val, pushed through and it builds again

src/Bitstream.v
@@ -9,107 +9,6 @@ Require Import Semantics.
 
 (* make some kind of type, convertible to val and strictval *)
 
-Inductive ext_val :=
-| ebit (b : bool)
-| eseq (l : list ext_val)
-| etup (l : list ext_val)
-| erec (f : list (string * ext_val))
-.
-
-Definition ext_val_rect_mut_full
-           (P : ext_val -> Type)
-           (Pl : list ext_val -> Type)
-           (Pp : string * ext_val -> Type)
-           (Plp : list (string * ext_val) -> Type)
-           (Hbit : forall b, P (ebit b))
-           (Hseq : forall l, Pl l -> P (eseq l))
-           (Htup : forall l, Pl l -> P (etup l))
-           (Hrec : forall f, Plp f -> P (erec f))
-           (Hnil : Pl nil)
-           (Hcons : forall e es, P e -> Pl es -> Pl (e :: es))
-           (Hpnil : Plp nil)
-           (Hpcons : forall se ses, Pp se -> Plp ses -> Plp (se :: ses))
-           (Hpair : forall s e, P e -> Pp (s,e))
-           (e : ext_val) : P e :=
-  let fix go e :=
-      let fix go_list es :=
-          match es as es_ return Pl es_ with
-          | nil => Hnil
-          | e :: es => Hcons e es (go e) (go_list es)
-          end in
-      let go_pair p :=
-          let '(s,e) := p in
-          Hpair s e (go e) in
-      let fix go_pair_list ps :=
-          match ps as ps_ return Plp ps_ with
-          | nil => Hpnil
-          | p :: ps => Hpcons p ps (go_pair p) (go_pair_list ps)
-          end in
-      match e with
-      | ebit b => Hbit b
-      | eseq l => Hseq l (go_list l)
-      | etup l => Htup l (go_list l)
-      | erec f => Hrec f (go_pair_list f)
-      end in go e.
-
-Definition ext_val_ind_mut
-           (P : ext_val -> Prop)
-           (Hbit : forall b, P (ebit b))
-           (Hseq : forall l, Forall P l -> P (eseq l))
-           (Htup : forall l, Forall P l -> P (etup l))
-           (Hrec : forall f, Forall P (map snd f) -> P (erec f))
-           (e : ext_val) : P e.
-  
-  eapply ext_val_rect_mut_full.
-  exact Hbit.
-  exact Hseq.
-  exact Htup.
-  exact Hrec.
-  econstructor.
-  intros. econstructor; eauto.
-  simpl. econstructor.
-  simpl. intros.
-  econstructor; eauto. exact X.
-  simpl. intros. assumption.
-Defined.
-
-Fixpoint to_val (e : ext_val) : val :=
-  let fix to_val_list_pair (ps : list (string * ext_val)) :=
-      match ps with
-      | nil => nil
-      | (s,t) :: ps => (s, to_val t) :: (to_val_list_pair ps)
-      end in
-  match e with
-  | ebit b => bit b
-  | eseq l => thunk_list (map to_val l)
-  | etup l => tuple (map to_val l)
-  | erec f => rec (to_val_list_pair f)
-  end.
-
-Fixpoint to_val_list_pair (ps : list (string * ext_val)) :=
-  match ps with
-  | nil => nil
-  | (s,t) :: ps => (s, to_val t) :: (to_val_list_pair ps)
-  end.
-
-Fixpoint to_sval (e : ext_val) : strictval :=
-  let fix to_sval_list_pair (ps : list (string * ext_val)) :=
-      match ps with
-      | nil => nil
-      | (s,t) :: ps => (s,to_sval t) :: (to_sval_list_pair ps)
-      end in
-  match e with
-  | ebit b => sbit b
-  | eseq l => strict_list (map to_sval l)
-  | etup l => stuple (map to_sval l)
-  | erec f => srec (to_sval_list_pair f)
-  end.
-
-Fixpoint to_sval_list_pair (ps : list (string * ext_val)) :=
-  match ps with
-  | nil => nil
-  | (s,t) :: ps => (s,to_sval t) :: (to_sval_list_pair ps)
-  end.
 
 Lemma map_snd_to_sval_lp :
   forall f,
@@ -282,6 +181,7 @@ Proof.
   inversion H. subst. eapply IHx in H2. congruence.
 Qed.
 
+(*
 Lemma n_bits_eval :
   forall n x ge TE E,
     n_bits n x ->
@@ -316,3 +216,4 @@ Proof.
   exact sempty.
 Qed.
 
+*)
